introduce unique

theories/typing/uninit.v
@@ -11,46 +11,33 @@ Section uninit.
   Program Definition uninit1: type unit :=
     {| pt_size := 1;  pt_own _ _ vl := ⌜∃v, vl = [v]⌝; |}%I.
   Next Obligation. move=> *. by iDestruct 1 as (?) "->". Qed.
-  Global Instance uninit1_send : Send uninit1. Proof. done. Qed.
+  Global Instance uninit1_send: Send uninit1. Proof. done. Qed.
 
-  Definition uninit n : type unit := <{const ()}> (array n uninit1).
+  Definition uninit n : type unit := <{unique}> (array n uninit1).
 
-  Local Notation tts := (@prepeat id _ ()).
-  Local Lemma pvec_unit_unique n x : x = tts n.
-  Proof.
-    move: x. elim n=> /=[|? IH] x; [by case x|]. case x=> [[]?]. f_equal. apply IH.
-  Qed.
-  Local Instance const_tt_tts_iso n : Iso (const ()) (const (tts n)).
-  Proof.
-    split; extensionality x; [|by case x]=>/=. symmetry. apply pvec_unit_unique.
-  Qed.
-
-  Lemma uninit_own' n vπd tid vl :
-    (array n uninit1).(ty_own) vπd tid vl ⊣⊢ ⌜length vl = n⌝.
-  Proof. move: vl vπd. elim: n=> /=[|n IH] vl [vπ ?]; iSplit.
-    - by iIntros ([_[_->]]).
-    - rewrite length_zero_iff_nil. iIntros (->). iExists (const ()). iPureIntro.
-      split; [|done]. extensionality π. simpl. by case (vπ π)=> [].
-    - iDestruct 1 as (? _ ??->[_[_[?->]]]) "H /=". rewrite IH. by iDestruct "H" as %->.
-    - case vl=> /=[|v vl']; iIntros (Eq); [done|]. iExists (const ((), tts n)).
-      iSplit. { iPureIntro. extensionality π. simpl. apply (pvec_unit_unique (S n)). }
-      iExists [v], vl'. rewrite IH. iPureIntro. split; [done|].
-      split; [|by move: Eq=> [=]]. exists (). split; by [|exists v].
-  Qed.
   Lemma uninit_own n vπd tid vl : (uninit n).(ty_own) vπd tid vl ⊣⊢ ⌜length vl = n⌝.
   Proof.
-    simpl. setoid_rewrite uninit_own'. iPureIntro. split; [by move=> [_[_->]]|]=> ->.
-    exists (const (tts n)). split; [|done]. extensionality π. by case (vπd.1 π).
+    move: vπd=> [??]. rewrite mod_ty_own. move: vl. elim: n=> [|n IH] vl.
+    - by rewrite mod_ty_own length_zero_iff_nil.
+    - rewrite mod_ty_own -/hrepeat -/xprod_ty. iSplit.
+      + iDestruct 1 as (??->[?[_[?->]]]) "H /=". rewrite IH. by iDestruct "H" as %->.
+      + case vl=> /=[|v vl']; iIntros ([=]). iExists [v], vl'. rewrite IH.
+        iPureIntro. split; [done|]. split; [|done]. exists (). split; by [|exists v].
+  Qed.
+
+  Lemma uninit_0_unit: uninit 0 ≡ unit_ty.
+  Proof.
+    split=>//; move=> [??]*; [rewrite !mod_ty_own|rewrite !mod_ty_shr];
+    by rewrite compose_assoc semi_iso.
   Qed.
 
   Lemma uninit_plus_prod E L m n :
-    eqtype E L (const ((), ())) (const ()) (uninit (m + n)) (uninit m * uninit n).
+    eqtype E L unique unique (uninit (m + n)) (uninit m * uninit n).
   Proof.
-    have [->->]: @const _ () ((), ()) =
-        prod_map (const ()) (const ()) ∘ pvsep ∘ const (tts (m + n)) ∧
-      @const _ (() * ()) () =
-        const () ∘ (curry pvapp ∘ prod_map (const (tts m)) (const (tts n))).
-    { split; extensionality x; by [case x|case x=>[[][]]]. }
+    have [->->]:
+      @unique (() → ()*()) _ = prod_map unique unique ∘ (@pvsep () m n) ∘ unique ∧
+      @unique (()*() → ()) _ = unique ∘ (curry (@pvapp () m n) ∘ prod_map unique unique).
+    { split; fun_ext; by [case|case=>[[][]]]. }
     eapply eqtype_trans. { apply mod_ty_outin, _. } eapply eqtype_trans.
     { apply array_plus_prod. } apply prod_eqtype; apply mod_ty_inout, _.
   Qed.
