theories/util/basic.v
@@ -4,7 +4,7 @@ From stdpp Require Import prelude.
 (** * Utility for Natural Numbers *)
 
 Lemma succ_le m n : S m ≤ n → ∃n', n = S n' ∧ m ≤ n'.
-Proof. move: n=> [|n'] => Le; [by inversion Le|exists n'; lia]. Qed.
+Proof. move: n=> [|n]=> Le; [|exists n]; lia. Qed.
 
 (** * Utility for Lists *)
 
@@ -16,48 +16,65 @@ Proof.
   split; [done|]. split; [|done]=>/=. by f_equal.
 Qed.
 
-(** * Utility for Empty_set *)
-
-Global Instance Empty_set_empty: Empty Type := Empty_set.
-Definition absurd {A} (x: ∅) : A := match x with end.
-
 (** * Utility for Point-Free Style *)
 
-Class SemiIso {A B} (f: A → B) (g: B → A) := semi_iso: g ∘ f = id.
-Class Iso {A B} (f: A → B) (g: B → A) := iso: g ∘ f = id ∧ f ∘ g = id.
+Ltac fun_ext := apply functional_extensionality.
 
-Global Instance iso_semi_iso `{@Iso A B f g} : SemiIso f g. Proof. apply iso. Qed.
-Global Instance iso_semi_iso' `{@Iso A B f g} : SemiIso g f. Proof. apply iso. Qed.
+Class SemiIso {A B} (f: A → B) (g: B → A) := semi_iso: g ∘ f = id.
+
+Class Iso {A B} (f: A → B) (g: B → A) := { iso:> SemiIso f g; iso':> SemiIso g f }.
+
 Global Instance iso_id {A} : Iso (@id A) id. Proof. done. Qed.
-Global Instance iso_flip `{@Iso A B f g} : Iso g f | 100. Proof. split; apply iso. Qed.
+
 Global Instance semi_iso_inj `{@SemiIso A B f g} : Inj (=) (=) f | 100.
 Proof.
   move=> x y Eq. have [<-<-]: (g ∘ f) x = x ∧ (g ∘ f) y = y.
   { by rewrite semi_iso. } by rewrite /= Eq.
 Qed.
 
-Lemma compose_assoc {A B C D} (f: A → B) (g: B → C) (h: C → D) :
-  h ∘ (g ∘ f) = (h ∘ g) ∘ f.
+Lemma compose_assoc {A B C D} (f: A → B) g (h: C → D) : h ∘ (g ∘ f) = (h ∘ g) ∘ f.
 Proof. done. Qed.
 
 Definition s_comb {A B C} (f: A → B → C) (g: A → B) x := (f x) (g x).
 Infix "⊛" := s_comb (left associativity, at level 50).
 
-Lemma surjective_pairing_fun {A B C} (f: A → B * C) :
-  f = (pair ∘ (fst ∘ f) ⊛ (snd ∘ f)).
-Proof. extensionality x. by rewrite /s_comb /compose -surjective_pairing. Qed.
+Lemma surjective_pairing_fun {A B C} (f: A → B * C) : f = (pair ∘ (fst ∘ f) ⊛ (snd ∘ f)).
+Proof. fun_ext=> ?. by rewrite /s_comb /compose -surjective_pairing. Qed.
 
 Definition prod_assoc {A B C} '((x, (y, z))) : (A * B) * C := ((x, y), z).
 Definition prod_assoc' {A B C} '(((x, y), z)) : A * (B * C) := (x, (y, z)).
 Global Instance prod_assoc_iso {A B C} : Iso (@prod_assoc A B C) prod_assoc'.
-Proof. split; extensionality xyz; by [case xyz=> [?[??]]|case xyz=> [[??]?]]. Qed.
+Proof. split; fun_ext; by [case=> [?[??]]|case=> [[??]?]]. Qed.
 
 Definition prod_left_id {A} '(((), x)) : A := x.
 Definition prod_left_id' {A} (x: A) := ((), x).
 Global Instance prod_left_id_iso {A} : Iso (@prod_left_id A) prod_left_id'.
-Proof. split; extensionality x; by [case x=> [[]?]|]. Qed.
+Proof. split; fun_ext; by [case=> [[]?]|]. Qed.
 
 Definition prod_right_id {A} '((x, ())) : A := x.
 Definition prod_right_id' {A} (x: A) := (x, ()).
 Global Instance prod_right_id_iso {A} : Iso (@prod_right_id A) prod_right_id'.
-Proof. split; extensionality x; by [case x=> [?[]]|]. Qed.
+Proof. split; fun_ext; by [case=> [?[]]|]. Qed.
+
+(* * Utility for Singleton Types *)
+
+Class Unique A := { unique: A; eq_unique: ∀x: A, x = unique }.
+
+Program Global Instance unit_unique: Unique () := {| unique := () |}.
+Next Obligation. by move=> []. Qed.
+
+Program Global Instance prod_unique `{Unique A, Unique B}
+  : Unique (A * B) := {| unique := (unique, unique) |}.
+Next Obligation. move=> ????. case=> [??]; f_equal; apply eq_unique. Qed.
+
+Program Global Instance fun_unique {B} `{Unique A}
+  : Unique (B → A) := {| unique := const unique |}.
+Next Obligation. move=> *. fun_ext=>/= ?. apply eq_unique. Qed.
+
+Global Instance unique_iso `{Unique A, Unique B} : @Iso A B unique unique.
+Proof. split; fun_ext=>/= ?; symmetry; apply eq_unique. Qed.
+
+(** * Utility for Empty_set *)
+
+Global Instance Empty_set_empty: Empty Type := Empty_set.
+Definition absurd {A} (x: ∅) : A := match x with end.
