theories/typing/array.v
@@ -28,18 +28,16 @@ Section array.
     eqtype E L pvsep (curry pvapp) (array (m + n) ty) (array m ty * array n ty).
   Proof.
     elim: m=> [|m Eq].
-    - have [->->]: @pvsep A 0 n = prod_map (const -[]) id ∘ prod_left_id' ∧
-        curry (@pvapp A 0 n) = prod_left_id ∘ prod_map (const ()) id.
-      { split; extensionality x; by [case x=> [[]?]|]. }
+    - have [->->]: @pvsep A 0 n = prod_map unique id ∘ prod_left_id' ∧
+        curry (@pvapp A 0 n) = prod_left_id ∘ prod_map unique id.
+      { split; fun_ext; by [case=> [[]?]|]. }
       eapply eqtype_trans; [apply eqtype_symm; apply prod_ty_left_id|].
-      apply prod_eqtype; [|done].
-      apply mod_ty_inout, functional_extensionality. by move=> [].
+      apply prod_eqtype; [|done]. apply mod_ty_inout, _.
     - have [->->]: @pvsep A (S m) n = prod_map prod_to_cons_prod id ∘
           prod_assoc ∘ prod_map id pvsep ∘ cons_prod_to_prod ∧
         curry (@pvapp A (S m) n) = prod_to_cons_prod ∘
           (prod_map id (curry pvapp) ∘ (prod_assoc' ∘ prod_map cons_prod_to_prod id)).
-      { split; extensionality x; [|by case x=> [[??]?]]. case x=> [? xl]/=.
-        by case (pvsep xl). }
+      { split; fun_ext; [|by case=> [[??]?]]. move=> [? xl]/=. by case (pvsep xl). }
       eapply eqtype_trans. { apply mod_ty_outin, _. } eapply eqtype_trans.
       { apply prod_eqtype; [done|apply Eq]. } eapply eqtype_trans.
       { apply prod_ty_assoc. } apply prod_eqtype; [apply mod_ty_inout, _|done].
